share/steel/examples/pulse/dice/l0/L0Crypto.fst
@@ -30,19 +30,18 @@ val derive_key_pair_spec
   (ikm: Seq.seq U8.t)
   (lbl_len: hkdf_lbl_len)
   (lbl: Seq.seq U8.t)
-  : elseq U8.t v32us & elseq U8.t v32us
+  : Seq.seq U8.t & Seq.seq U8.t (* should be length 32 *)
 
 ```pulse
 fn derive_key_pair
-  (pub : A.larray U8.t (US.v v32us))
-  (priv: A.larray U8.t (US.v v32us))
+  (pub : A.larray U8.t 32)
+  (priv: A.larray U8.t 32)
   (ikm_len: hkdf_ikm_len) 
   (ikm: A.array U8.t)
   (lbl_len: hkdf_lbl_len) 
   (lbl: A.array U8.t)
   (#ikm_perm #lbl_perm:perm)
-  (#_pub_seq #_priv_seq:erased (elseq U8.t v32us))
-  (#ikm_seq #lbl_seq:erased (Seq.seq U8.t))
+  (#_pub_seq #_priv_seq #ikm_seq #lbl_seq:erased (Seq.seq U8.t))
   requires (
     A.pts_to pub full_perm _pub_seq ** 
     A.pts_to priv full_perm _priv_seq ** 
@@ -68,7 +67,7 @@ let derive_DeviceID_spec
   (cdi: Seq.seq U8.t) (* should be length 32 *)
   (l0_label_DeviceID_len: hkdf_lbl_len)
   (l0_label_DeviceID: Seq.seq U8.t)
-: elseq U8.t v32us & elseq U8.t v32us
+: Seq.seq U8.t & Seq.seq U8.t (* should be length 32 *)
 = let cdigest = spec_hash alg cdi in
   derive_key_pair_spec
     (* ikm *) dig_len cdigest
@@ -77,13 +76,12 @@ let derive_DeviceID_spec
 ```pulse 
 fn derive_DeviceID
   (alg:alg_t)
-  (deviceID_pub:A.larray U8.t (US.v v32us))
-  (deviceID_priv:A.larray U8.t (US.v v32us))
+  (deviceID_pub:A.larray U8.t 32)
+  (deviceID_priv:A.larray U8.t 32)
   (cdi:A.larray U8.t (US.v dice_digest_len))
   (deviceID_label_len:hkdf_lbl_len)
   (deviceID_label:A.larray U8.t (US.v deviceID_label_len))
-  (#cdi0 #deviceID_label0:erased (Seq.seq U8.t))
-  (#deviceID_pub0 #deviceID_priv0:erased (elseq U8.t v32us))
+  (#cdi0 #deviceID_label0 #deviceID_pub0 #deviceID_priv0: Ghost.erased (Seq.seq U8.t))
   requires (
     A.pts_to cdi full_perm cdi0 **
     A.pts_to deviceID_label full_perm deviceID_label0 **
@@ -94,7 +92,7 @@ fn derive_DeviceID
   ensures (
     A.pts_to cdi full_perm cdi0 **
     A.pts_to deviceID_label full_perm deviceID_label0 **
-    (exists (deviceID_pub1 deviceID_priv1:elseq U8.t v32us). (
+    (exists (deviceID_pub1:Seq.seq U8.t) (deviceID_priv1:Seq.seq U8.t). (
         A.pts_to deviceID_pub full_perm deviceID_pub1 **
         A.pts_to deviceID_priv full_perm deviceID_priv1 **
         pure (
@@ -106,7 +104,7 @@ fn derive_DeviceID
   )
 {
   let cdigest = new_array 0uy (digest_len alg);
-  hacl_hash alg dice_digest_len cdi cdigest;
+  hacl_hash alg cdi dice_digest_len cdigest;
 
   derive_key_pair
     deviceID_pub deviceID_priv
@@ -125,7 +123,7 @@ let derive_AliasKey_spec
   (fwid: Seq.seq U8.t) (* should be length 32 *)
   (l0_label_AliasKey_len: hkdf_lbl_len)
   (l0_label_AliasKey: Seq.seq U8.t)
-: elseq U8.t v32us & elseq U8.t v32us
+: Seq.seq U8.t & Seq.seq U8.t (* should be length 32 *)
 = let cdigest = spec_hash alg cdi in
   let adigest = spec_hmac alg cdigest fwid in
   derive_key_pair_spec
@@ -135,14 +133,13 @@ let derive_AliasKey_spec
 ```pulse 
 fn derive_AliasKey
   (alg:alg_t)
-  (aliasKey_pub: A.larray U8.t (US.v v32us))
-  (aliasKey_priv: A.larray U8.t (US.v v32us))
+  (aliasKey_pub: A.larray U8.t 32)
+  (aliasKey_priv: A.larray U8.t 32)
   (cdi: A.larray U8.t (US.v dice_digest_len))
-  (fwid: A.larray U8.t (US.v v32us))
+  (fwid: A.larray U8.t 32)
   (aliasKey_label_len: hkdf_lbl_len)
   (aliasKey_label: A.larray U8.t (US.v aliasKey_label_len))
-  (#cdi0 #fwid0 #aliasKey_label0:erased (Seq.seq U8.t))
-  (#aliasKey_pub0 #aliasKey_priv0:erased (elseq U8.t v32us))
+  (#cdi0 #fwid0 #aliasKey_label0 #aliasKey_pub0 #aliasKey_priv0: Ghost.erased (Seq.seq U8.t))
   requires (
     A.pts_to cdi full_perm cdi0 **
     A.pts_to fwid full_perm fwid0 **
@@ -155,7 +152,7 @@ fn derive_AliasKey
     A.pts_to cdi full_perm cdi0 **
     A.pts_to fwid full_perm fwid0 **
     A.pts_to aliasKey_label full_perm aliasKey_label0 **
-    (exists (aliasKey_pub1 aliasKey_priv1:elseq U8.t v32us). (
+    (exists (aliasKey_pub1:Seq.seq U8.t) (aliasKey_priv1:Seq.seq U8.t). (
         A.pts_to aliasKey_pub full_perm aliasKey_pub1 **
         A.pts_to aliasKey_priv full_perm aliasKey_priv1 **
         pure (
@@ -170,9 +167,9 @@ fn derive_AliasKey
   let cdigest = new_array 0uy (digest_len alg);
   let adigest = new_array 0uy (digest_len alg);
 
-  hacl_hash alg dice_digest_len cdi cdigest;
+  hacl_hash alg cdi dice_digest_len cdigest;
   is_hashable_len_32;
-  hacl_hmac alg adigest cdigest (digest_len alg) fwid v32us;
+  hacl_hmac alg adigest cdigest (digest_len alg) fwid 32sz;
 
   derive_key_pair
     aliasKey_pub aliasKey_priv
@@ -195,9 +192,8 @@ let derive_AuthKeyID_spec
 fn derive_AuthKeyID
   (alg:alg_t)
   (authKeyID: A.larray U8.t (US.v (digest_len alg)))
-  (deviceID_pub: A.larray U8.t (US.v v32us))
-  (#authKeyID0:erased (Seq.seq U8.t))
-  (#deviceID_pub0:erased (elseq U8.t v32us))
+  (deviceID_pub: A.larray U8.t 32)
+  (#authKeyID0 #deviceID_pub0: Ghost.erased (Seq.seq U8.t))
   requires (
     A.pts_to deviceID_pub full_perm deviceID_pub0 **
     A.pts_to authKeyID full_perm authKeyID0 
@@ -211,7 +207,7 @@ fn derive_AuthKeyID
   )
 {
   is_hashable_len_32;
-  hacl_hash alg v32us deviceID_pub authKeyID #full_perm #(coerce v32us deviceID_pub0);
+  hacl_hash alg deviceID_pub 32sz authKeyID;
   ()
 }
 ```
